Phi_System/IDE_CP_Reasoning1.thy
@@ -463,6 +463,42 @@ lemma [\<phi>reason 1000]:
   unfolding Pass_Embedded_Reasoning'_def by blast
 
 
+subsection \<open>Semantic Type of Multiple Values\<close>
+
+lemma [\<phi>reason 1200 for \<open>\<phi>_Have_Types (\<lambda>vs. ?R vs\<heavy_comma> ?x \<Ztypecolon> \<v>\<a>\<l>[\<phi>V_fst vs] ?T) _\<close>]:
+  \<open> \<phi>SemType (x \<Ztypecolon> T) TY
+\<Longrightarrow> \<phi>_Have_Types (\<lambda>vs. R vs) TYs
+\<Longrightarrow> \<phi>_Have_Types (\<lambda>vs. R (\<phi>V_snd vs)\<heavy_comma> x \<Ztypecolon> \<v>\<a>\<l>[\<phi>V_fst vs] T) (TY#TYs)\<close>
+  unfolding \<phi>_Have_Types_def Well_Typed_Vals_def \<phi>arg_forall \<phi>SemType_def subset_iff
+  by (clarsimp simp add: to_vals_prod_def to_vals_VAL_def Val_inhabited_rewr)
+
+lemma [\<phi>reason 1200]:
+  \<open> \<phi>SemType (x \<Ztypecolon> T) TY
+\<Longrightarrow> \<phi>_Have_Types (\<lambda>vs. R\<heavy_comma> x \<Ztypecolon> \<v>\<a>\<l>[vs] T) [TY]\<close>
+  unfolding \<phi>_Have_Types_def Well_Typed_Vals_def \<phi>arg_forall \<phi>SemType_def subset_iff
+  by (clarsimp simp add: to_vals_prod_def to_vals_VAL_def Val_inhabited_rewr)
+
+lemma [\<phi>reason 1200]:
+  \<open> \<phi>_Have_Types R TYs
+\<Longrightarrow> \<phi>_Have_Types (\<lambda>vs. R vs\<heavy_comma> S) TYs\<close>
+  unfolding \<phi>_Have_Types_def Well_Typed_Vals_def by clarsimp
+
+lemma [\<phi>reason 2000]:
+  \<open> \<phi>_Have_Types (\<lambda>_::unit \<phi>arg. Void) []\<close>
+  unfolding \<phi>_Have_Types_def Well_Typed_Vals_def to_vals_unit_def by clarsimp
+
+lemma [\<phi>reason 1020 except \<open>\<phi>_Have_Types (\<lambda>vs. ?A vs\<heavy_comma> ?B vs) _\<close>]:
+  \<open> \<phi>_Have_Types (\<lambda>vs. Void\<heavy_comma> R vs) TYs
+\<Longrightarrow> \<phi>_Have_Types R TYs\<close>
+  unfolding \<phi>_Have_Types_def Well_Typed_Vals_def by clarsimp
+
+lemma [\<phi>reason 1000]:
+  \<open> FAIL TEXT(\<open>Fail to infer the semantic type of\<close> R)
+\<Longrightarrow> \<phi>_Have_Types R TYs\<close>
+  unfolding \<phi>_Have_Types_def Well_Typed_Vals_def by clarsimp
+
+
+
 
 section \<open>Declaration of Large Processes\<close>
 
